examples/pseudo_bool/array/compilation/cnfCompileScript.sml
@@ -6,6 +6,6 @@ open preamble compilationLib cnfProgTheory
 val _ = new_theory "cnfCompile"
 
 val cnf_compiled = save_thm("cnf_compiled",
-  compile_x64 "cnf" main_prog_def);
+  compile_x64 "cake_pb_cnf" main_prog_def);
 
 val _ = export_theory ();
